backend/RTL.v
@@ -250,8 +250,6 @@ Inductive step: state -> trace -> state -> Prop :=
       find_function ros rs = Some fd ->
       funsig fd = sig ->
       Mem.free m stk 0 f.(fn_stacksize) = Some m' ->
-
-
       step (State s f (Vptr stk Ptrofs.zero) pc rs m)
         E0 (Callstate s fd rs##args m' (fn_stack_requirements id))
   | exec_Ibuiltin:
@@ -341,7 +339,7 @@ Inductive initial_state (p: program): state -> Prop :=
       Genv.find_symbol ge p.(prog_main) = Some b ->
       Genv.find_funct_ptr ge b = Some f ->
       funsig f = signature_main ->
-      initial_state p (Callstate nil f nil m0 (fn_stack_requirements (prog_main p))).
+      initial_state p (Callstate nil f nil (Mem.push_stage m0) (fn_stack_requirements (prog_main p))).
 
 (** A final state is a [Returnstate] with an empty call stack. *)
 
